LambdaS5/coq/LjsInitEnv.v
@@ -2595,7 +2595,7 @@ expr_if
  (expr_string "DeclEnvRec"))
 (expr_if
  (expr_op1 unary_op_not
-  (expr_op2 binary_op_has_property (expr_id "context") (expr_id "id")))
+  (expr_op2 binary_op_has_own_property (expr_id "context") (expr_id "id")))
  (expr_app (expr_id "%DeclEnvAddBinding")
   [expr_id "context";
    expr_id "id";
